wip

src/OeufCompcertSimulations.v
@@ -118,10 +118,202 @@ Proof.
 Qed.
 
 (* RTLgen, RTLgenproof *)
+Inductive rtl_final_state (p : RTL.program) : RTL.state -> value -> Prop :=
+| rtl_final_state_intro: forall v v' m,
+    value_inject (Genv.globalenv p) m v v' ->
+    rtl_final_state p (RTL.Returnstate nil v' m) v.
+
+Definition RTL_semantics (p : RTL.program) :=
+  Semantics RTL.step (RTL.initial_state p) (rtl_final_state p) (Genv.globalenv p).
+
+Lemma rtl_final_states :
+  forall prog tprog,
+    RTLgen.transl_program prog = OK tprog ->
+    forall st st' v,
+      RTLgenproof.match_states st st' ->
+      cminorsel_final_state prog st v ->
+      rtl_final_state tprog st' v.
+Proof.
+  intros.
+  inv H1. inv H0. inv MS.
+  eapply value_inject_mem_extends in MEXT; eauto.
+  econstructor; eauto.
+  eapply value_inject_swap_ge; eauto.
+  intros. eapply RTLgenproof.function_ptr_translated in H; eauto.
+  break_exists; break_and; eexists; eauto.
+  intros.
+  intros. eapply RTLgenproof.symbols_preserved in H; eauto.
+  erewrite H; eauto.
+Qed.
+
+Lemma star_star :
+  forall {F V S} step (ge : Genv.t F V) (s : S) t s',
+    Smallstep.star step ge s t s' ->
+    star step ge s t s'.
+Proof.
+  induction 1; intros.
+  eapply star_refl; eauto.
+  subst. econstructor; eauto.
+Qed.
+
+Lemma plus_plus :
+  forall {F V S} step (ge : Genv.t F V) (s : S) t s',
+    Smallstep.plus step ge s t s' ->
+    plus step ge s t s'.
+Proof.
+  intros. inv H.
+  econstructor; eauto.
+  eapply star_star; eauto.
+Qed.
+
+Lemma rtl_transf_program_correct :
+  forall (prog : CminorSel.program) (tprog : RTL.program),
+    RTLgen.transl_program prog = OK tprog ->
+    forward_simulation (CminorSel_semantics prog) (RTL_semantics tprog).
+Proof.
+  intros. eapply forward_simulation_star_wf.
+  eapply RTLgenproof.transl_initial_states; eauto.
+  eapply rtl_final_states; eauto.
+  Focus 2.
+  intros.
+  eapply RTLgenproof.transl_step_correct in H0; eauto.
+  break_exists. repeat break_and; destruct H0; repeat break_and.
+  eexists; split; auto; try left; try eassumption.
+  simpl.
+  eapply plus_plus; eauto.
+  eexists; split; auto; try right; try split; try eassumption.
+  eapply star_star; eauto.
+  eapply RTLgenproof.lt_state_wf.
+Qed.
+
 (* Tailcall, Tailcallproof *)
+Lemma tailcall_final_states :
+  forall prog st st' v,
+    Tailcallproof.match_states st st' ->
+    rtl_final_state prog st v ->
+    rtl_final_state (Tailcall.transf_program prog) st' v.
+Proof.
+  intros.
+  inv H0. inv H.
+  inv H5.
+  eapply value_inject_mem_extends in H8; eauto.
+  econstructor; eauto.
+  eapply value_inject_swap_ge; eauto.
+  intros.
+  eapply Tailcallproof.funct_ptr_translated in H2; eauto.
+  intros. erewrite Tailcallproof.symbols_preserved; eauto.
+Qed.
+
+Lemma tailcall_transf_program_correct :
+  forall (prog tprog : RTL.program),
+    Tailcall.transf_program prog = tprog ->
+    forward_simulation (RTL_semantics prog) (RTL_semantics tprog).
+Proof.
+  intros. subst tprog.
+  eapply forward_simulation_star.
+  intros. eapply Tailcallproof.transf_initial_states; eauto.
+  intros. eapply tailcall_final_states; eauto.
+  intros. simpl in *. 
+  eapply Tailcallproof.transf_step_correct in H0; eauto.
+  destruct H0; repeat break_exists; repeat break_and.
+  left. eexists; split; eauto. eapply plus_one; eauto.
+  right. subst. split. eauto. split; eauto.
+Qed.
+
 (* Inlining, Inliningproof *)
+Lemma inlining_final_states :
+  forall prog tprog st st' v,
+    Inlining.transf_program prog = OK tprog ->
+    Inliningproof.match_states prog st st' ->
+    rtl_final_state prog st v ->
+    rtl_final_state tprog st' v.
+Proof.
+  intros.
+  inv H1. inv H0.
+  
+(*  intros. erewrite Inliningproof.symbols_preserved; eauto.
+  eapply Inliningproof.function_ptr_translated in H2; eauto.*)
+Admitted.
+
+Lemma inlining_transf_program_correct :
+  forall (prog tprog : RTL.program),
+    Inlining.transf_program prog = OK tprog ->
+    forward_simulation (RTL_semantics prog) (RTL_semantics tprog).
+Proof.
+  intros. 
+  eapply forward_simulation_star.
+  intros. eapply Inliningproof.transf_initial_states; eauto.
+  intros. eapply inlining_final_states; eauto.
+  intros. simpl in *.
+  eapply Inliningproof.step_simulation in H0; eauto.
+  destruct H0. break_exists. break_and.
+  left. eexists.  split; eauto. eapply plus_plus; eauto.
+  right. repeat break_and; repeat split; eauto.
+Qed.
+
 (* Renumber, Renumberproof *)
+Lemma renumber_final_states :
+  forall prog st st' v,
+    Renumberproof.match_states st st' ->
+    rtl_final_state prog st v ->
+    rtl_final_state (Renumber.transf_program prog) st' v.
+Proof.
+  intros.
+  inv H0. inv H.
+  inv STACKS.
+  econstructor; eauto.
+  eapply value_inject_swap_ge; eauto.
+  intros.
+  eapply Renumberproof.function_ptr_translated in H2; eauto.
+  intros. erewrite Renumberproof.symbols_preserved; eauto.
+Qed.
+
+Lemma renumber_transf_program_correct :
+  forall (prog tprog : RTL.program),
+    Renumber.transf_program prog = tprog ->
+    forward_simulation (RTL_semantics prog) (RTL_semantics tprog).
+Proof.
+  intros. subst tprog.
+  eapply forward_simulation_step.
+  intros. eapply Renumberproof.transf_initial_states; eauto.
+  intros. eapply renumber_final_states; eauto.
+  intros. simpl in *.
+  eapply Renumberproof.step_simulation in H0; eauto.
+Qed.
+
 (* Constprop, Constpropproof *)
+Lemma constprop_final_states :
+  forall prog n st st' v,
+    Constpropproof.match_states prog n st st' ->
+    rtl_final_state prog st v ->
+    rtl_final_state (Constprop.transf_program prog) st' v.
+Proof.
+  intros.
+  inv H0. inv H.
+  inv H7.
+  econstructor; eauto.
+  eapply value_inject_mem_extends in H1; eauto.
+  eapply value_inject_swap_ge; eauto.
+  intros.
+  eapply Constpropproof.function_ptr_translated in H2; eauto.
+  intros. erewrite Constpropproof.symbols_preserved; eauto.
+Qed.
+
+Lemma constprop_transf_program_correct :
+  forall (prog tprog : RTL.program),
+    Constprop.transf_program prog = tprog ->
+    forward_simulation (RTL_semantics prog) (RTL_semantics tprog).
+Proof.
+  intros. subst tprog.
+  eapply forward_simulation_star.
+  admit. (* weird thing with nats here *)
+  intros. eapply constprop_final_states; eauto.
+  intros. simpl in *.
+  eapply Constpropproof.transf_step_correct in H0; eauto.
+Admitted.
+
+
+
 (* CSE, CSEproof *)
 (* Deadcode, Deadcodeproof *)
 (* Unusedglob, Unusedglobproof *)
